steel/Zeta.Steel.Main.fsti
@@ -21,58 +21,47 @@ module SA = Zeta.SeqAux
 module MR = Steel.MonotonicReference
 #push-options "--ide_id_info_off"
 
-
-let grows (#a:Type) :Preorder.preorder (erased (Seq.seq a))
-  = let open FStar.Seq in
-    fun (s1 s2:erased (seq a)) ->
-      length s1 <= length s2 /\
-      (forall (i:nat).{:pattern (Seq.index s1 i) \/ (Seq.index s2 i)}
-         i < length s1 ==> index s1 i == index s2 i)
-
-let log = Seq.seq log_entry_base
-let elog = erased log
-
-/// This should be a MR.ghost_ref
-let monotonic_log_t = MR.ref elog grows
-
-let mlog_refs_t = Map.t thread_id monotonic_log_t
-
 let thread_inv (t: V.thread_state_t)
                (logref: AEH.log_ref)
-               (mlogref: monotonic_log_t)
   : vprop
   = exists_ (fun tsm ->
        V.thread_state_inv t tsm `star`
-       G.pts_to logref half (M.committed_entries tsm) `star`
-       MR.pts_to mlogref half tsm.M.processed_entries)
+       G.pts_to logref half (M.committed_entries tsm))
 
 noeq
-type thread_state (logrefs:AEH.log_refs_t)
-                  (mlogrefs:mlog_refs_t) =
+type thread_state (logrefs:AEH.log_refs_t) =
 {
   tid: tid;
   tsm: V.thread_state_t;
   logref: AEH.log_ref;
-  mlogref: monotonic_log_t;
-  lock : Lock.lock (thread_inv tsm logref mlogref);
+  lock : Lock.lock (thread_inv tsm logref);
   properties : squash (
-    logref == Map.sel logrefs tid /\
-    mlogref == Map.sel mlogrefs tid
+    logref == Map.sel logrefs tid
   );
 }
 
-let all_threads_t logrefs mlogrefs =
-  a:A.array (thread_state logrefs mlogrefs) {
+let all_threads_t logrefs =
+  a:A.array (thread_state logrefs) {
       A.length a == U32.v n_threads
   }
 
 noeq
 type top_level_state = {
   logrefs : erased AEH.log_refs_t;
-  mlogrefs : erased mlog_refs_t; //should be erased
-  all_threads : all_threads_t logrefs mlogrefs;
-  epoch_hashes: AEH.aggregate_epoch_hashes logrefs;
+  all_threads : all_threads_t (reveal logrefs);
+  epoch_hashes: AEH.aggregate_epoch_hashes (reveal logrefs);
 }
+
+
+let thread_has_processed (t:top_level_state)
+                         (tid:tid)
+                         (entries:AEH.log) =
+    AEH.thread_has_processed t.epoch_hashes.mlogs tid entries
+
+let all_threads_have_processed (t:top_level_state)
+                               (entries:AEH.all_processed_entries) =
+    AEH.all_threads_have_processed t.epoch_hashes.mlogs entries
+
 
 /// TODO: a fractional permission variant of Steel.ST.Array
 val array_pts_to (#t:Type0)
@@ -81,7 +70,7 @@ val array_pts_to (#t:Type0)
                  (v:Seq.seq t)
   : vprop
 
-let tid_positions_ok #l #m (all_threads: Seq.seq (thread_state l m))
+let tid_positions_ok #l (all_threads: Seq.seq (thread_state l))
   : prop
   = forall (i:SA.seq_index all_threads).
         let si = Seq.index all_threads i in
@@ -94,75 +83,54 @@ let core_inv (t:top_level_state)
       array_pts_to t.all_threads perm v `star`
       pure (tid_positions_ok v)))
 
-let initial_inv (t:top_level_state)
-  : vprop
-  = core_inv t `star`
-    AEH.forall_threads (fun (tid:thread_id) ->
-      MR.pts_to (Map.sel t.mlogrefs tid) half Seq.empty)
-
 // This creates a Zeta instance
 val init (_:unit)
-  : STT top_level_state emp initial_inv
+  : STT top_level_state emp core_inv
 
 val verify_entries (t:top_level_state)
-                   (tid:thread_id)
-                   (#log_bytes:erased bytes) (len: U32.t) (input:A.array U8.t { A.length input == U32.v len })
-                   (out_len: U32.t) (output:A.array U8.t { A.length output == U32.v out_len })
-                   (#entries:elog) (mlogref:monotonic_log_t { Map.sel t.mlogrefs tid == mlogref })
+                   (tid:tid)
+                   (#log_bytes:erased bytes)
+                   (len: U32.t)
+                   (input:larray U8.t len)
+                   (out_len: U32.t)
+                   (output:larray U8.t out_len)
   : STT (option U32.t) //bool & U32.t & erased (Seq.seq log_entry_base))
     (core_inv t `star`
      A.pts_to input log_bytes `star`
-     exists_ (A.pts_to output) `star`
-     MR.pts_to mlogref half entries)
+     exists_ (A.pts_to output))
     (fun res ->
       core_inv t `star`
       A.pts_to input log_bytes `star`
       (match res, V.parse_log log_bytes with
        | None, _ ->
-         exists_ (A.pts_to output) `star`
-         exists_ (MR.pts_to mlogref half)
+         exists_ (A.pts_to output)
 
        | Some _, None ->
          pure False
 
        | Some n_out, Some entries' ->
+         exists_ (fun entries -> //this is a little weak: It doesn't prevent the thread from silently adding some more entries to the log
+                              //we could give a 1/4 permission to the logref to the client to allow them to correlate the initial
+                              //state, rather than just existentially quantifying it here
          exists_ (fun out_bytes ->
            A.pts_to output out_bytes `star`
-           MR.pts_to mlogref half (entries `Seq.append` entries') `star`
            pure (
              let tsm0 = M.verify_model (M.init_thread_state_model tid) entries in
              let tsm1 = M.verify_model tsm0 entries' in
              out_bytes == M.bytes_of_app_results (M.delta_app_results tsm0 tsm1) /\
-             U32.v n_out == Seq.length out_bytes))))
+             U32.v n_out == Seq.length out_bytes /\
+             thread_has_processed t tid (entries `Seq.append` entries'))))))
 
-let prefix_of (#a:Type) (s0 s1:Seq.seq a)
-  : prop
-  = let open FStar.Seq in
-    length s0 <= length s1 /\
-    Seq.slice s1 0 (length s0) == s0
-
-let snapshot (r:monotonic_log_t) (s:log) =
-  MR.witnessed r (fun s' -> prefix_of s s')
-
-let run_threads (logs:Map.t tid log) (tid:tid)
-  : M.thread_state_model
-  = M.verify_model (M.init_thread_state_model tid) (Map.sel logs tid)
-
-let tid_logs (a:M.all_logs) (tid:tid) =
-  Seq.index a (U16.v tid)
-
-val max_certified_epoch (t:top_level_state)
-                        (all_logs: erased M.all_logs)
+val max_certified_epoch (logs:erased AEH.all_processed_entries)
+                        (t:top_level_state)
   : ST M.epoch_id
     (core_inv t)
     (fun _ -> core_inv t)
-    (requires
-      forall (tid:tid). let lr_i = Map.sel t.mlogrefs tid in
-                   snapshot lr_i (tid_logs all_logs tid))
+    (requires all_threads_have_processed t logs)
     (ensures fun max ->
       forall (eid:M.epoch_id).
          U32.v eid <= U32.v max ==>
-         M.epoch_is_certified all_logs eid)
+         M.epoch_is_certified logs eid)
 
 //From this, we should connect back to the semantic
 //proof and show that the entries are sequentially consistent up to eid
